binary-trie: complete proof by proving unaffected query.

binary-trie/Trie.v
@@ -1,4 +1,6 @@
 Require Import Coq.Lists.List.
+Require Import Coq.Classes.DecidableClass.
+Require Import Bool Coq.Init.Specif.
 
 Section Trie.
 
@@ -71,31 +73,114 @@ Fixpoint search (bs : bits) (t : trie) : option A :=
      end
   end.
 
-Inductive IsNode : trie -> Prop :=
-| isnode: forall l r v, IsNode (Node l r v).
-
-Theorem new_IsNode :
-  forall (t : trie), IsNode (new t).
+Lemma new_is_node :
+  forall (t : trie), exists l r v, new t = Node l r v.
 Proof.
+  intro t.
   unfold new.
-  destruct t; constructor.
+  destruct t; eauto.
 Qed.
 
-Theorem insert_then_search :
-  forall (bs : bits) (v : A) (t : trie),
-    IsNode t -> search bs (insert bs v t) = Some v.
+Lemma search_leaf :
+  forall (bs : bits), search bs Leaf = None.
 Proof.
-  intro bs.
-  induction bs.
-  - intros. inversion H; subst.
-    unfold search, insert. auto.
-  - intros. inversion H; subst.
-    unfold insert. unfold search.
-    fold insert. fold search.
+  intros. induction bs; unfold search; auto.
+Qed.
+
+Hint Resolve search_leaf.
+
+Inductive BitsEq : bits -> bits -> Prop :=
+| eq_nil : BitsEq nil nil
+| eq_cons : forall (b : bool) (b1 b2 : bits),
+    BitsEq b1 b2 -> BitsEq (b :: b1) (b :: b2).
+
+Ltac invert H := inversion H; clear H; subst.
+
+Ltac invert_new t :=
+  let H := fresh in assert (H: exists l r v, new t = Node l r v) by apply new_is_node;
+  destruct H; destruct H; destruct H; rewrite H.
+
+(* Surprisingly, Coq's standard library doesn't have these useful two lemmas,
+   so they bother ourselves to prove these two lemmas ;o *)
+Lemma bool_decidable :
+  forall (a b : bool), Decidable.decidable (a = b).
+Proof.
+  intros. unfold Decidable.decidable.
+  assert ( {a = b} + {a <> b} ). { apply bool_dec. }
+  destruct H; tauto.
+Qed.
+
+Lemma bool_neq_is_neg :
+  forall (a b : bool), a <> b -> a = negb b.
+Proof.
+  intros.
+  destruct a; destruct b; auto.
+  exfalso. apply H. auto.
+Qed.
+
+(* Lemmas on not BitsEq. *)
+Lemma bits_neq_cons :
+  forall a b bs1 bs2,
+    ~ BitsEq (a :: bs1) (b :: bs2) -> a <> b \/ ~ BitsEq bs1 bs2.
+Proof.
+  intros. apply Decidable.not_and. apply bool_decidable.
+  intros [H1 H2]. subst. apply H.
+  apply eq_cons. apply H2.
+Qed.
+
+Lemma bits_neq_nil :
+  forall bs,
+    ~ BitsEq nil bs -> exists b bs', bs = b :: bs'.
+Proof.
+  intros.
+  assert (bs <> nil). { intros contra. apply H. subst. constructor. }
+  destruct bs.
+  - exfalso. apply H0. auto.
+  - eauto.
+Qed.
+
+(* Theorem 1: If we are querying a trie after inserting with the same bits,
+     we expect to get the updated value. *)
+Theorem insert_affact_eq_search :
+  forall (bs1 bs2 : bits) (v : A) (t : trie),
+    BitsEq bs1 bs2 -> search bs2 (insert bs1 v (new t)) = Some v.
+Proof.
+  intro bs1.
+  induction bs1; intros; invert H.
+  - unfold search, insert, new.
+    destruct t; auto.
+  - unfold search, insert.
+    invert_new t.
+    fold search. fold insert.
     destruct a.
-    + apply IHbs. apply new_IsNode.
-    + assert (IsNode (new r)). { apply new_IsNode. }
-      apply IHbs; auto.
+    + apply IHbs1. apply H3.
+    + apply IHbs1; auto.
+Qed.
+
+(* Theorem 2: If we are querying a updated trie with different bits, the
+     result should be unchanged. *)
+Theorem insert_unaffect_neq_search :
+  forall (bs1 bs2 : bits) (v : A) (t : trie),
+    ~ (BitsEq bs1 bs2) -> search bs2 t = search bs2 (insert bs1 v (new t)).
+Proof.
+  intros bs1.
+  induction bs1; intros.
+  - unfold search, insert; fold search.
+    apply bits_neq_nil in H.
+    destruct H as [b [bs2' H0]]. subst.
+    unfold search; fold search.
+    destruct t; simpl; destruct b; auto.
+  - unfold search, insert; fold search; fold insert.
+    destruct bs2.
+    + unfold search.
+      destruct t; simpl; destruct a; auto.
+    + apply bits_neq_cons in H. destruct H.
+      * apply bool_neq_is_neg in H.
+        destruct b; simpl in H; subst; destruct t; simpl; auto.
+      * unfold search; fold search.
+        assert (Node Leaf Leaf None = new Leaf). { auto. }
+        destruct a; destruct b; destruct t; simpl; try rewrite H0; auto;
+        rewrite <- (search_leaf bs2); apply IHbs1; auto.
 Qed.
 
 End Trie.
